Makefile
@@ -1,0 +1,8 @@
+# Needs FSTAR_HOME to point to FStar's root directory
+
+FSTAR=$(FSTAR_HOME)/bin/fstar.exe
+
+verify-bloom:
+	make -C bloom-filter/ verify
+
+verify: verify-bloom
